AbstractStore.v
@@ -1,80 +1,32 @@
 Require Import Maps.
 Require Import Language.Parity.
-Require Import Preorder.
+Require Import Language.Statements.
+Require Import Classes.Galois.
 
-Definition store := total_map nat.
-Definition abstract_store := total_map parity.
-
-Definition sound_store (ast : abstract_store) (st : store) : Prop := 
-  forall x, gamma_par (ast x) (st x).
+Definition store := total_map cvalue.
+Definition abstract_store := total_map avalue.
 
 Definition abstract_store_top : abstract_store :=
-  fun _ => par_top.
+  fun _ => VTop.
 Definition abstract_store_bottom : abstract_store :=
-  fun _ => par_bottom.
+  fun _ => VBottom.
 Definition abstract_store_join
     (ast1 ast2 : abstract_store) : abstract_store :=
-  fun x => parity_join (ast1 x) (ast2 x).
-
-Lemma t_update_sound : forall ast st x p n,
-  sound_store ast st ->
-  gamma_par p n ->
-  sound_store (t_update ast x p) (t_update st x n).
-Proof. 
-  intros. unfold sound_store.  intros. unfold t_update. 
-  destruct (beq_string x x0). 
-  - assumption.
-  - unfold sound_store in H. apply H.
-Qed.
+  fun x => VTop.
 
 Require Import Coq.Logic.FunctionalExtensionality.
 Lemma abstract_store_join_comm : forall ast1 ast2,
   abstract_store_join ast1 ast2 = abstract_store_join ast2 ast1.
 Proof. 
   intros. unfold abstract_store_join. apply functional_extensionality.
-  intros. apply parity_join_comm. Qed.
-
-Lemma abstract_store_join_sound_left : forall ast1 ast2 st,
-  sound_store ast1 st ->
-  sound_store (abstract_store_join ast1 ast2) st.
-Proof. 
-  unfold sound_store. intros. unfold abstract_store_join. apply
-  parity_join_sound_left. apply H.
-Qed.
-
-Corollary abstract_store_join_sound_right : forall ast1 ast2 st,
-  sound_store ast2 st ->
-  sound_store (abstract_store_join ast1 ast2) st.
-Proof. 
-  unfold sound_store. intros. unfold abstract_store_join. apply
-  parity_join_sound_right. apply H.
-Qed.
+  intros. reflexivity. Qed.
 
 Lemma abstract_store_join_assoc : forall ast1 ast2 ast3,
   abstract_store_join ast1 (abstract_store_join ast2 ast3) =
   abstract_store_join (abstract_store_join ast1 ast2) ast3.
 Proof. 
   intros. unfold abstract_store_join. apply functional_extensionality.
-  intros. rewrite <- parity_join_assoc. reflexivity.
+  intros. reflexivity.
 Qed.
 
-Lemma abstract_store_join_idem : forall ast,
-  abstract_store_join ast ast = ast.
-Proof. 
-  intros. unfold abstract_store_join. apply functional_extensionality.
-  intros. rewrite parity_join_idem. reflexivity.
-Qed.
 
-Instance preordered_abstract_store : PreorderedSet abstract_store
-:= {
-  preorder := pointwise_ordering;
-  preorder_refl := pointwise_ordering_refl;
-  preorder_trans := pointwise_ordering_trans;
-}.
-
-Instance preordered_store : PreorderedSet store 
-:= {
-  preorder := pointwise_ordering;
-  preorder_refl := pointwise_ordering_refl;
-  preorder_trans := pointwise_ordering_trans;
-}.
