Language/Statements.v
@@ -8,33 +8,27 @@ Inductive cvalue : Type :=
 
 Inductive avalue : Type :=
   | VParity : parity -> avalue
-  | VAbstrBool : abstr_bool -> avalue.
-  
-Inductive value : Type :=
-  | VAbs : avalue -> value
-  | VConc : cvalue -> value.
+  | VAbstrBool : abstr_bool -> avalue
+  | VTop : avalue
+  | VBottom : avalue.
 
 (* expand on the above *)
 
-Inductive aexp : Type :=
-  | ANum : nat -> aexp
-  | AVar : string -> aexp
-  | APlus : aexp -> aexp -> aexp
-  | AMult : aexp -> aexp -> aexp.
-
-Inductive bexp : Type :=
-  | BTrue : bexp
-  | BFalse : bexp
-  | BEq : aexp -> aexp -> bexp
-  | BLe : aexp -> aexp -> bexp
-  | BNot : bexp -> bexp
-  | BAnd : bexp -> bexp -> bexp.
+Inductive expr : Type :=
+  | EVal : cvalue -> expr
+  | EVar : string -> expr
+  | EPlus : expr -> expr -> expr
+  | EMult : expr -> expr -> expr
+  | EEq : expr -> expr -> expr
+  | ELe : expr -> expr -> expr
+  | ENot : expr -> expr
+  | EAnd : expr -> expr -> expr.
 
 Inductive com : Type :=
   | CSkip : com
   | CSeq : com -> com -> com
-  | CAss : string -> aexp -> com
-  | CIf  : bexp -> com -> com -> com
+  | CAss : string -> expr -> com
+  | CIf  : expr -> com -> com -> com
   | CTryCatch : com -> com -> com
   | CFail : com.
 
@@ -47,12 +41,6 @@ Notation "x '::=' a" :=
     (CAss x a) (at level 60) : com_scope.
 Notation "'try' c1 'catch' c2" :=
     (CTryCatch c1 c2) (at level 70) : com_scope.
-
-Definition plus_op (v1 v2 : cvalue) : option cvalue :=
-  match v1, v2 with
-  |  VNat x, VNat y =>  Some (VNat (plus x y))
-  | _, _ => None
-  end.
 
 
 (* zoek naar papers over 'auto' in coq, en het maken van proofs
