Soundness.v
@@ -6,7 +6,9 @@ Require Import AbstractBool.
 Require Import AbstractStore.
 Require Import AbstractInterpreter.
 Require Import ConcreteInterpreter.
+Require Import PreorderedSet.
 Require Import Galois.
+Require Import GaloisInstances.
 Require Import Joinable.
 Require Import Statements.
 Require Import Maps.
@@ -18,11 +20,44 @@ Require Import State.
 Create HintDb soundness.
 
 Tactic Notation "pairs" := unfold gamma_pairs; simpl; split;auto; try reflexivity.
+Hint Extern 4 => pairs.
 
 Definition sound {A B A' B' : Type} 
   `{Galois B A} `{Galois B' A'}
   (f : B->B') (f' : A->A') :=
   forall b a, gamma a b -> gamma (f' a) (f b).
+Hint Unfold sound.
+  
+Definition sound_store (ast : abstract_store) (st : store) : Prop := 
+  forall x, gamma (ast x) (st x).
+Hint Unfold sound_store.
+
+Lemma t_update_sound : forall ast st x p n,
+  sound_store ast st ->
+  gamma p n ->
+  sound_store (t_update ast x p) (t_update st x n).
+Proof. 
+  intros. unfold sound_store.  intros. unfold t_update. 
+  destruct (beq_string x x0). 
+  - assumption.
+  - unfold sound_store in H. apply H.
+Qed.
+
+Lemma abstract_store_join_sound_left : forall ast1 ast2 st,
+  sound_store ast1 st ->
+  sound_store (abstract_store_join ast1 ast2) st.
+Proof. 
+  unfold sound_store. intros. unfold abstract_store_join. 
+  constructor.
+Qed.
+
+Corollary abstract_store_join_sound_right : forall ast1 ast2 st,
+  sound_store ast2 st ->
+  sound_store (abstract_store_join ast1 ast2) st.
+Proof.
+  unfold sound_store. intros. unfold abstract_store_join. 
+  constructor.
+Qed.
 
 Lemma bind_state_sound {A A' B B'} 
 `{Galois A A', Galois B B'}
@@ -52,6 +87,7 @@ Qed.
 Hint Resolve bind_state_sound.
 
 Tactic Notation "bind" := apply bind_state_sound;auto;try reflexivity.
+Hint Extern 4 => bind.
 
 Lemma sound_parity_plus :
   sound plus parity_plus.
@@ -60,6 +96,7 @@ Proof. intros ? ? ? ? ? ?.
   destruct a, a0; simpl in *; try tauto;
   auto using even_even_plus, odd_plus_r, odd_plus_l, odd_even_plus.
 Qed.
+Hint Extern 5 => apply sound_parity_plus.
 
 Lemma sound_parity_mult :
   sound mult parity_mult.
@@ -68,6 +105,7 @@ Proof.
   destruct a, a0; simpl in *; try tauto; 
   auto using even_mult_l, even_mult_r, odd_mult.
 Qed.
+Hint Extern 5 => apply sound_parity_mult.
 
 Lemma sound_parity_eq :
   sound Nat.eqb parity_eq.
@@ -79,6 +117,7 @@ Proof.
   - apply Bool.Is_true_eq_true in H1. apply Nat.eqb_eq in H1. subst.
     eauto using not_even_and_odd.
 Qed.
+Hint Extern 5 => apply sound_parity_eq.
 
 Lemma sound_ab_and :
   sound andb and_ab.
@@ -86,6 +125,7 @@ Proof.
   unfold sound. simpl. unfold gamma_fun. intros.
   destruct b, b0, a, a0; simpl in *; tauto.
 Qed.
+Hint Extern 5 => apply sound_ab_and.
 
 Lemma sound_ab_or :
   sound orb or_ab.
@@ -93,6 +133,7 @@ Proof.
   unfold sound. simpl. unfold gamma_fun. intros.
   destruct b, b0, a, a0; simpl in *; tauto.
 Qed.
+Hint Extern 5 => apply sound_ab_or.
 
 Lemma sound_ab_neg :
   sound negb neg_ab.
@@ -100,88 +141,79 @@ Proof.
   unfold sound. simpl. unfold gamma_fun. intros.
   destruct b, a; simpl in *; tauto.
 Qed.
+Hint Extern 5 => apply sound_ab_neg.
 
-Theorem eval_aexp_sound :
-  forall a, sound (concrete_aexp a) (abstract_aexp a).
+Lemma gamma_extract_n_n : forall v,
+  gamma (extract v) v.
+Proof.
+  destruct v.
+  - simpl. apply gamma_par_extract_n_n.
+  - simpl. destruct b; simpl. reflexivity.
+    unfold not. intros contra. inversion contra.
+Qed.
+Hint Extern 5 => apply gamma_extract_n_n.
+
+Lemma ensure_par_sound : 
+  sound ensure_nat ensure_par.
+Proof.
+  unfold sound. intros b a Hgamma.
+  simpl. unfold gamma_fun. intros ast st Hstore. simpl.
+  destruct a, b; try inversion Hgamma; pairs.
+Qed.
+Hint Extern 5 => apply ensure_par_sound.
+
+Lemma ensure_abool_sound :
+  sound ensure_bool ensure_abool.
+Proof.
+  unfold sound. intros b c Hgamma.
+  simpl. unfold gamma_fun. intros ast st Hstore. simpl.
+  destruct c, b; try inversion Hgamma; pairs.
+Qed.
+Hint Extern 5 => apply ensure_abool_sound.
+  
+Hint Unfold gamma_fun.
+Hint Unfold gamma_store.
+Theorem eval_expr_sound :
+  forall a, sound (eval_expr a) (eval_expr_abstract a).
 Proof.
   intros.
   unfold sound. simpl.
   induction a.
-  - (* ANum *) simpl. pairs. apply gamma_par_extract_n_n.
-  - (* AVar *) simpl. pairs. unfold gamma_store in H. apply H.
-  - (* APlus *) simpl in *. intros st ast H. bind.
+  - (* ENum *) simpl. pairs. 
+  - (* EVar *) simpl. pairs. unfold gamma_store in H. apply H.
+  - (* EPlus *) simpl in *. intros st ast H. bind. 
     unfold sound. intros n p Hgamma. simpl. unfold gamma_fun. 
     intros ast' st'. intros Hstore. simpl. bind.
     unfold sound. intros n' p' Hgamma'. simpl. unfold gamma_fun.
-    intros ast'' st'' Hgamma''. simpl. pairs.
-    apply sound_parity_plus; assumption.
+    intros ast'' st'' Hgamma''. simpl. bind.
+    unfold sound. intros n'' p'' Hgamman''p''. simpl. unfold gamma_fun.
+    intros ast''' st''' Hgamma_store'''. bind.
   - (* AMult *) intros st ast Hstore. simpl. 
     bind. intros n p Hpar. simpl. unfold gamma_fun. intros ast' st' Hstore'.
     simpl. bind.
     unfold sound. intros n' p' Hpar'. simpl. unfold gamma_fun.
-    intros ast'' st'' Hstore''. simpl. pairs.
-    apply sound_parity_mult; assumption.
+    intros ast'' st'' Hstore''. simpl. bind.
+    unfold sound. intros. simpl. auto.
+  - (* EEq *)
+    intros. simpl. bind. unfold sound. intros. simpl. unfold gamma_fun.
+    intros. simpl. bind. unfold sound. intros. simpl. unfold gamma_fun.
+    intros. simpl. bind. unfold sound. intros. simpl. unfold gamma_fun.
+    intros. simpl. bind.
+  - (* ELe *)
+    intros. simpl. bind. unfold sound. intros. simpl. unfold gamma_fun.
+    intros. simpl. bind. unfold sound. intros. simpl. unfold gamma_fun.
+    intros. simpl. bind. unfold sound. intros. simpl. unfold gamma_fun.
+    intros. simpl. bind.
+  - (* ENot *)
+    intros. simpl. bind. unfold sound. intros. simpl. unfold gamma_fun.
+    intros. simpl. bind.
+  - (* EAnd *)
+    intros. simpl. bind. unfold sound. intros. simpl. unfold gamma_fun.
+    intros. simpl. bind. unfold sound. intros. simpl. unfold gamma_fun.
+    intros. simpl. bind. unfold sound. intros. simpl. unfold gamma_fun.
+    intros. simpl. bind.
 Qed.
-
-Lemma eval_bexp_beq_sound : forall n n',
-sound (eval_bexp (BEq n n')) (beval_abstract (BEq n n')).
-Proof. 
-  unfold sound. simpl. intros a a' st ast Hstore. simpl. 
-  bind. apply eval_aexp_sound.
-  unfold sound. intros n p Hpar. simpl. unfold gamma_fun.
-  intros ast' st' Hstore'. simpl. bind. 
-  unfold sound. intros n' p' Hpar'. simpl. unfold gamma_fun.
-  apply eval_aexp_sound. assumption.
-  intros ast'' st'' Hstore''. simpl. pairs.
-  apply sound_parity_eq. assumption. assumption.
-Qed.
-
-Lemma eval_bexp_ble_sound : forall n n', 
-sound (eval_bexp (BLe n n')) (beval_abstract (BLe n n')).
-Proof. 
-  intros a a'. simpl. bind. apply eval_aexp_sound.
-  unfold sound. intros n p Hpar. simpl. unfold gamma_fun. intros ast st Hstore.
-  simpl. bind. unfold sound. intros n' p' Hpar'. apply eval_aexp_sound. assumption. 
-  intros ast' st' Hstore'. simpl. pairs; auto.
-Qed.
-
-Lemma eval_bexp_not_sound : forall b,
-sound (eval_bexp b) (beval_abstract b) ->
-sound (eval_bexp (BNot b)) (beval_abstract (BNot b)).
-Proof. 
-  intros b H.
-  unfold sound. intros st ast Hstore. simpl. bind.
-  unfold sound. intros b' ab Hbool. simpl. unfold gamma_fun. 
-  intros aast' st' Hstore'. pairs.
-  apply sound_ab_neg. apply Hbool.
-Qed.
-
-Lemma eval_bexp_and_sound : forall b1 b2,
-sound (eval_bexp b1) (beval_abstract b1) ->
-sound (eval_bexp b2) (beval_abstract b2) ->
-sound (eval_bexp (BAnd b1 b2)) (beval_abstract (BAnd b1 b2)).
-Proof. 
-  intros b1 b2 H1 H2. unfold sound. intros st ast Hstore.
-  simpl. bind. unfold sound. intros b ab Hbool. simpl. unfold gamma_fun.
-  intros ast' st' Hstore'. simpl. bind.
-  unfold sound. intros b' ab' Hbool'. simpl. unfold gamma_fun.
-  intros ast'' st'' Hstore''. simpl. pairs.
-  - apply sound_ab_and; assumption.
-Qed.
-
-Theorem eval_bexp_sound :
-  forall b, sound (eval_bexp b) (beval_abstract b).
-Proof.
-  induction b.
-  - simpl. unfold sound. intros st ast Hstore. simpl. 
-    pairs.
-  - simpl. unfold sound. intros st ast Hstore. simpl.
-    pairs.
-  - apply eval_bexp_beq_sound; apply eval_aexp_sound.
-  - apply eval_bexp_ble_sound; apply eval_aexp_sound.
-  - apply eval_bexp_not_sound. apply IHb.
-  - apply eval_bexp_and_sound; assumption.
-Qed.
+Hint Resolve eval_expr_sound.
 
 Lemma sound_seq : forall c1 c2,
   sound (ceval c1) (ceval_abstract c1) ->
@@ -199,11 +231,9 @@ Lemma sound_assignment : forall x a,
   sound (ceval (CAss x a)) (ceval_abstract (CAss x a)).
 Proof. 
   intros. unfold sound. intros. bind.
-  - apply eval_aexp_sound.
-  - simpl. unfold sound. intros. simpl. unfold gamma_fun. intros.
-    simpl. unfold gamma_pairs. simpl. split.
-    + constructor.
-    + unfold gamma_store. intros x'. apply t_update_sound; assumption.
+  simpl. unfold sound. intros. simpl. unfold gamma_fun. intros.
+  simpl. unfold gamma_pairs. simpl. split; auto.
+  unfold gamma_store. intros x'. apply t_update_sound; assumption.
 Qed.
 
 Hint Resolve sound_assignment.
@@ -213,29 +243,30 @@ Lemma sound_if : forall b c1 c2,
   sound (ceval c2) (ceval_abstract c2) ->
   sound (ceval (CIf b c1 c2)) (ceval_abstract (CIf b c1 c2)).
 Proof. 
-  intros. simpl. bind.
-  { apply eval_bexp_sound. }
-  unfold sound. intros. simpl.
-  unfold eval_if_abstract. unfold eval_if. destruct a.
-  - (* ab_true *) destruct b0. unfold gamma_fun; intros. apply H. apply H2. inversion H1.
+  intros e c1 c2 H1 H2. simpl. bind.
+  unfold sound. intros cv av Hgamma. simpl.
+  unfold gamma_fun. intros. bind. unfold sound. intros.
+  unfold eval_if_abstract. unfold eval_if. simpl in *. destruct a0.
+  - (* ab_true *) destruct b0. unfold gamma_fun; intros. auto. 
+    inversion H0.
   - (* ab_false *) destruct b0. 
-    + (* true, contradiction *) simpl in *. unfold not in H1. 
-      exfalso. apply H1. reflexivity.
-    + (* false *) unfold gamma_fun;intros. apply H0. apply H2.
+    + (* true, contradiction *) simpl in *. unfold not in H0. 
+      exfalso. apply H0. reflexivity.
+    + (* false *) unfold gamma_fun;intros. apply H2. apply H3.
   - (* ab_top *) destruct b0.
     + (* true *)
       assert (preorder (ceval_abstract c1) (join_op (ceval_abstract c1) (ceval_abstract c2))).
       apply join_upper_bound_left.
       unfold gamma_fun; intros.
-      simpl in H2. inversion H2; subst. 
-      eapply widen. apply H4. auto.
+      simpl in H3. inversion H3; subst. 
+      eapply widen. apply H5. auto.
     + (* false *) 
       assert (preorder (ceval_abstract c2) (join_op (ceval_abstract c1) (ceval_abstract c2))).
       apply join_upper_bound_right.
       unfold gamma_fun; intros.
-      simpl in H2. inversion H2; subst.
-      eapply widen. apply H4. auto.
-  - (* ab_bottom *) inversion H1.
+      simpl in H3. inversion H3; subst.
+      eapply widen. apply H5. auto.
+  - (* ab_bottom *) inversion H0.
 Qed.
 
 Hint Resolve sound_if.
@@ -274,7 +305,7 @@ Hint Resolve sound_fail.
 Lemma sound_skip :
   sound (ceval SKIP) (ceval_abstract SKIP).
 Proof.
-  simpl. split; auto. simpl. reflexivity.
+  simpl. split; auto. 
 Qed.
 
 Hint Resolve sound_skip.
