Classes/Galois.v
@@ -1,0 +1,11 @@
+Require Import PreorderedSet.
+
+Class Galois (A B : Type) 
+`{PreorderedSet B} : Type :=
+{
+  gamma : B -> A -> Prop;
+  gamma_monotone : monotone gamma;
+
+}.
+Arguments Build_Galois A B {_ _ _}.
+Arguments gamma {_ _ _ _}.
