Language/AbstractBool.v
@@ -1,5 +1,4 @@
 Require Import Coq.Bool.Bool.
-Require Import Preorder.
 
 (** * Definition *)
 
@@ -22,13 +21,6 @@ Proof.
   intros. destruct a, b, c; try constructor; try inversion H0; try inversion H.
 Qed.
 
-Instance preorder_ab : PreorderedSet abstr_bool :=
-{
-  preorder := ab_le;
-  preorder_refl := ab_le_refl;
-  preorder_trans := ab_le_trans;
-}.
-
 Definition gamma_bool (ab: abstr_bool) (b : bool) : Prop :=
   match ab with
   | ab_true   => Is_true b
@@ -43,12 +35,7 @@ Definition extract_bool (b: bool) : abstr_bool :=
   | false => ab_false
   end.
 
-Lemma gamma_bool_monotone : monotone gamma_bool.
-Proof.
-  unfold monotone. intros b1 b2 ?.
-  destruct b1, b2; constructor; intros; destruct x; simpl in *; 
-    try inversion H0; try inversion H; try tauto. 
-Qed.
+
 
 
 (** * Operations *)
